pulse/lib/pulse/core/PulseCore.MemoryAlt.fst
@@ -1,0 +1,684 @@
+(*
+   Copyright 2024 Microsoft Research
+
+   Licensed under the Apache License, Version 2.0 (the "License");
+   you may not use this file except in compliance with the License.
+   You may obtain a copy of the License at
+
+       http://www.apache.org/licenses/LICENSE-2.0
+
+   Unless required by applicable law or agreed to in writing, software
+   distributed under the License is distributed on an "AS IS" BASIS,
+   WITHOUT WARRANTIES OR CONDITIONS OF ANY KIND, either express or implied.
+   See the License for the specific language governing permissions and
+   limitations under the License.
+*)
+
+module PulseCore.MemoryAlt
+open FStar.Ghost
+open FStar.PCM
+module PST = PulseCore.HoareStateMonad
+module U = FStar.Universe
+module S = FStar.Set
+module CM = FStar.Algebra.CommMonoid
+module H = PulseCore.HeapSig
+module E = PulseCore.HeapExtension
+module B = PulseCore.BaseHeapSig
+/// This module adds memory invariants to the heap to expose the
+/// final interface for Pulse's PCM-based memory model.
+
+(**** Basic memory properties *)
+let small_sig : H.heap_sig u#(a + 1) = E.extend (B.base_heap u#a)
+let sig : H.heap_sig u#(a + 2) = E.extend small_sig
+(** Abstract type of memories *)
+let mem  : Type u#(a + 3) = sig.mem
+
+let is_ghost_action (m0 m1:mem u#a) : prop = sig.is_ghost_action m0 m1
+
+let ghost_action_preorder (_:unit)
+: Lemma (FStar.Preorder.preorder_rel is_ghost_action)
+= sig.is_ghost_action_preorder ()
+ 
+(**** Separation logic *)
+
+(** The type of separation logic propositions. Based on Steel.Heap.slprop *)
+let slprop : Type u#(a + 3) = sig.slprop
+
+let big_slprop : Type u#(a + 2) = sig.bprop
+let cm_big_slprop : CM.cm big_slprop = H.cm_slprop small_sig
+let down (s:slprop u#a) : big_slprop u#a = sig.down s
+let up (s:big_slprop u#a) : slprop u#a = sig.up s
+let up_big_is_big (b:big_slprop) : Lemma (is_big (up b)) = sig.up_down b
+
+let small_slprop : Type u#(a + 1) = small_sig.bprop
+let cm_small_slprop : CM.cm small_slprop = H.cm_slprop B.base_heap
+let down2 (s:slprop u#a) : small_slprop u#a = small_sig.down (sig.down s)
+let up2 (s:small_slprop u#a) : slprop u#a = sig.up (small_sig.up s)
+let small_is_also_big (s:slprop)
+: Lemma (is_small s ==> is_big s)
+= sig.up_down (small_sig.up (small_sig.down (down s)))
+
+let up2_small_is_small (s:small_slprop)
+: Lemma (is_small (up2 s))
+= calc (==) {
+    up2 (down2 (up2 s));
+  (==) {}
+    up2 (down2 (sig.up (small_sig.up s)));
+  (==) {}
+    up2 (small_sig.down (sig.down (sig.up (small_sig.up s))));
+  (==) { sig.up_down (small_sig.up s) }
+    up2 (small_sig.down (small_sig.up s));
+  (==) { small_sig.up_down s }
+    up2 s;
+  }
+
+(** Interpreting mem assertions as memory predicates *)
+let interp (p:slprop u#a) (m:mem u#a) : prop = H.interpret p m
+
+let equiv (p1 p2:slprop u#a) : prop = p1 == p2
+
+(**
+  An extensional equivalence principle for slprop
+ *)
+
+let slprop_extensionality (p q:slprop u#a)
+: Lemma
+    (requires p `equiv` q)
+    (ensures p == q)
+= ()
+
+let slprop_equiv_refl (p:slprop)
+: Lemma (p `equiv` p)
+        [SMTPat (equiv p p)]
+= ()
+          
+(** A memory maps a [ref]erence to its associated value *)
+let core_ref : Type u#0 = PulseCore.Heap.core_ref
+
+(** [null] is a specific reference, that is not associated to any value
+*)
+let core_ref_null : core_ref = PulseCore.Heap.core_ref_null
+
+let core_ref_is_null (r:core_ref)
+: b:bool { b <==> r == core_ref_null }
+= PulseCore.Heap.core_ref_is_null r
+
+assume
+val emp_up
+        (h:H.heap_sig)
+: Lemma ((E.extend h).emp == (E.extend h).up h.emp)
+
+assume
+val pure_up
+        (h:H.heap_sig)
+        (p:prop)
+: Lemma ((E.extend h).pure p == (E.extend h).up (h.pure p))
+
+let emp_is_small () 
+: Lemma (is_small sig.emp)
+= emp_up B.base_heap;
+  emp_up small_sig;
+  small_sig.up_down B.base_heap.emp;
+  sig.up_down small_sig.emp
+
+let pure_is_small (p:prop) 
+: Lemma (is_small (sig.pure p))
+= pure_up B.base_heap p;
+  pure_up small_sig p;
+  small_sig.up_down (B.base_heap.pure p);
+  sig.up_down (small_sig.pure p)
+
+let emp
+: vprop u#a
+= emp_is_small(); sig.emp
+
+let pure (p:prop)
+: vprop u#a
+= pure_is_small p; sig.pure p
+
+let star  (p1 p2:slprop u#a)
+: slprop u#a
+= sig.star p1 p2
+
+module F = FStar.FunctionalExtensionality
+let h_exists (#a:Type u#b) (f: (a -> slprop u#a))
+: slprop u#a
+= H.exists_ sig #a (fun x -> f x)
+
+(***** Properties of separation logic equivalence *)
+let emp_unit (p:slprop)
+: Lemma (p `equiv` (p `star` emp))
+= sig.emp_unit p
+
+let pure_equiv (p q:prop)
+: Lemma ((p <==> q) ==> (pure p `equiv` pure q))
+= FStar.PropositionalExtensionality.apply p q
+
+let pure_true_emp (_:unit)
+: Lemma (pure True `equiv` emp)
+= sig.pure_true_emp ()
+
+(***** Properties of the separating conjunction *)
+let star_commutative (p1 p2:slprop)
+: Lemma ((p1 `star` p2) `equiv` (p2 `star` p1))
+= sig.star_commutative p1 p2
+
+let star_associative (p1 p2 p3:slprop)
+: Lemma ((p1 `star` (p2 `star` p3))
+          `equiv`
+          ((p1 `star` p2) `star` p3))
+= sig.star_associative p1 p2 p3
+
+let star_congruence (p1 p2 p3 p4:slprop)
+  : Lemma (requires p1 `equiv` p3 /\ p2 `equiv` p4)
+          (ensures (p1 `star` p2) `equiv` (p3 `star` p4))
+= ()
+
+let big_star_congruence (p1 p2:big_vprop u#a)
+: Lemma (is_big (p1 `star` p2))
+= admit()
+
+let big_exists_congruence (#a:Type u#a) (p:a -> slprop u#b)
+: Lemma
+  (requires forall x. is_big (p x))
+  (ensures is_big (h_exists p))
+= admit()
+
+let small_star_congruence (p1 p2:vprop u#a)
+: Lemma (is_small (p1 `star` p2))
+= admit()
+
+let small_exists_congruence (#a:Type u#a) (p:a -> slprop u#b)
+: Lemma
+  (requires forall x. is_small (p x))
+  (ensures is_small (h_exists p))
+= admit()
+
+let h_exists_equiv (#a:Type) (p q : a -> slprop)
+: Lemma
+    (requires (forall x. p x `equiv` q x))
+    (ensures (h_exists p == h_exists q))
+= admit()
+
+let up_emp_big ()
+: Lemma (up cm_big_slprop.unit == emp)
+= admit()
+
+let down_emp_big ()
+: Lemma (down emp == cm_big_slprop.unit)
+= admit()
+
+let up_star_big (p q:big_slprop)
+: Lemma (up (p `cm_big_slprop.mult` q) == up p `star` up q)
+= admit()
+
+let down_star_big (p q:big_vprop)
+: Lemma (down (p `star` q) == down p `cm_big_slprop.mult` down q)
+= admit()
+
+let up2_emp ()
+: Lemma (up2 cm_small_slprop.unit == emp)
+= admit()
+
+let down2_emp ()
+: Lemma (down2 emp == cm_small_slprop.unit)
+= admit()
+
+let up2_star (p q:small_slprop)
+: Lemma (up2 (p `cm_small_slprop.mult` q) == up2 p `star` up2 q)
+= admit()
+
+let down2_star (p q:vprop)
+: Lemma (down2 (p `star` q) == down2 p `cm_small_slprop.mult` down2 q)
+= admit()
+
+(**** Memory invariants *)
+
+(** Invariants have a name *)
+let iname : eqtype = sig.iname
+let inames_ok (e:inames) (m:mem) : prop = H.inames_ok e m
+
+(** The empty set of invariants is always empty *)
+let inames_ok_empty (m:mem)
+: Lemma (ensures inames_ok Set.empty m)
+          [SMTPat (inames_ok Set.empty m)]
+= ()
+
+(**
+  This separation logic proposition asserts that all the invariants whose names are in [e]
+  are in effect and satisfied on the heap inside the memory [m]
+*)
+let mem_invariant (e:inames) (m:mem u#a)
+: slprop u#a
+= sig.mem_invariant e m
+
+let full_mem_pred: mem -> prop = sig.full_mem_pred 
+
+let iref : Type0 = sig.iref
+
+let iname_of (i:iref) : GTot iname = sig.iname_of i
+
+let inv (i:iref) (p:slprop u#a) : slprop u#a = sig.inv i p
+
+#push-options "--print_universes --print_implicits"
+let coerce_action
+    (#a:Type u#x)
+    (#mg:bool)
+    (#ex:inames)
+    (#pre:slprop u#a)
+    (#post:a -> GTot (slprop u#a))
+    (act:H._action_except (sig u#a) a mg ex pre post)
+    (pre':slprop u#a)
+    (post':a -> slprop u#a)
+    (_:squash (pre == reveal pre' /\ (forall x. post x == reveal (post' x))))
+: _pst_action_except a mg ex pre' post'
+= fun frame m0 -> act frame m0 
+
+let dup_inv (e:inames) (i:iref) (p:slprop u#a)
+: pst_ghost_action_except unit e 
+    (inv i p) 
+    (fun _ -> inv i p `star` inv i p)
+= E.dup_inv #(small_sig u#a) e i p
+
+let new_invariant (e:inames) (p:slprop { is_big p })
+: pst_ghost_action_except iref e
+    p
+    (fun i -> inv i p)
+= E.new_invariant #(small_sig u#a) e p 
+
+let with_invariant (#a:Type u#x)
+                   (#fp:slprop u#a)
+                   (#fp':a -> slprop u#a)
+                   (#opened_invariants:inames)
+                   (#p:slprop u#a)
+                   (#maybe_ghost:bool)
+                   (i:iref{not (mem_inv opened_invariants i)})
+                   (f:_pst_action_except a maybe_ghost
+                        (add_inv opened_invariants i) 
+                        (p `star` fp)
+                        (fun x -> p `star` fp' x))
+: _pst_action_except a maybe_ghost opened_invariants 
+      (inv i p `star` fp)
+      (fun x -> inv i p `star` fp' x)
+= E.with_invariant #(small_sig u#a) #a #fp #fp' #opened_invariants #p #maybe_ghost i f
+
+(*
+val distinct_invariants_have_distinct_names
+      (e:inames)
+      (p:slprop u#m)
+      (q:slprop u#m { p =!= q })
+      (i j: iref)
+: pst_ghost_action_except u#0 u#m 
+    (squash (iname_of i =!= iname_of j))
+    e 
+    (inv i p `star` inv j q)
+    (fun _ -> inv i p `star` inv j q)
+
+val invariant_name_identifies_invariant
+      (e:inames)
+      (p q:slprop u#m)
+      (i:iref)
+      (j:iref { iname_of i == iname_of j } )
+: pst_ghost_action_except (squash (p == q /\ i == j)) e
+   (inv i p `star` inv j q)
+   (fun _ -> inv i p `star` inv j q)
+   
+let rec all_live (ctx:list iref) =
+  match ctx with
+  | [] -> emp
+  | hd::tl -> live hd `star` all_live tl
+
+let fresh_wrt (ctx:list iref)
+              (i:iref)
+  = forall i'. List.Tot.memP i' ctx ==> iname_of i' <> iname_of i
+
+val fresh_invariant (e:inames) (p:big_vprop u#m) (ctx:list iref)
+  : pst_ghost_action_except (i:iref { fresh_wrt ctx i }) e
+       (p `star` all_live ctx)
+       (fun i -> inv i p)
+*)
+
+(* Some generic actions and combinators *)
+
+val pst_frame (#a:Type)
+              (#maybe_ghost:bool)
+              (#opened_invariants:inames)
+              (#pre:slprop)
+              (#post:a -> slprop)
+              (frame:slprop)
+              ($f:_pst_action_except a maybe_ghost opened_invariants pre post)
+  : _pst_action_except a maybe_ghost opened_invariants (pre `star` frame) (fun x -> post x `star` frame)
+
+
+val witness_h_exists (#opened_invariants:_) (#a:_) (p:a -> slprop)
+  : pst_ghost_action_except (erased a) opened_invariants
+           (h_exists p)
+           (fun x -> p x)
+
+val intro_exists (#opened_invariants:_) (#a:_) (p:a -> slprop) (x:erased a)
+  : pst_ghost_action_except unit opened_invariants
+           (p x)
+           (fun _ -> h_exists p)
+
+val lift_h_exists (#opened_invariants:_) (#a:_) (p:a -> slprop)
+  : pst_ghost_action_except unit opened_invariants
+           (h_exists p)
+           (fun _a -> h_exists #(U.raise_t a) (U.lift_dom p))
+
+val elim_pure (#opened_invariants:_) (p:prop)
+  : pst_ghost_action_except (u:unit{p}) opened_invariants (pure p) (fun _ -> emp)
+
+val intro_pure (#opened_invariants:_) (p:prop) (_:squash p)
+  : pst_ghost_action_except unit opened_invariants emp (fun _ -> pure p)
+
+val drop (#opened_invariants:_) (p:slprop)
+  : pst_ghost_action_except unit opened_invariants p (fun _ -> emp)
+
+let non_info a = x:erased a -> y:a { reveal x == y}
+
+val lift_ghost
+      (#a:Type)
+      #opened_invariants #p #q
+      (ni_a:non_info a)
+      (f:erased (pst_ghost_action_except a opened_invariants p q))
+  : pst_ghost_action_except a opened_invariants p q
+
+(* Concrete references to "small" types *)
+val pts_to (#a:Type u#a) (#pcm:_) (r:ref a pcm) (v:a) : vprop u#a
+
+val sel_action (#a:Type u#a) (#pcm:_) (e:inames) (r:ref a pcm) (v0:erased a)
+  : pst_action_except (v:a{compatible pcm v0 v}) e (pts_to r v0) (fun _ -> pts_to r v0)
+
+val upd_action (#a:Type u#a) (#pcm:_) (e:inames)
+               (r:ref a pcm)
+               (v0:FStar.Ghost.erased a)
+               (v1:a {FStar.PCM.frame_preserving pcm v0 v1 /\ pcm.refine v1})
+  : pst_action_except unit e (pts_to r v0) (fun _ -> pts_to r v1)
+
+val free_action (#a:Type u#a) (#pcm:pcm a) (e:inames)
+                (r:ref a pcm) (x:FStar.Ghost.erased a{FStar.PCM.exclusive pcm x /\ pcm.refine pcm.FStar.PCM.p.one})
+  : pst_action_except unit e (pts_to r x) (fun _ -> pts_to r pcm.FStar.PCM.p.one)
+
+(** Splitting a permission on a composite resource into two separate permissions *)
+val split_action
+  (#a:Type u#a)
+  (#pcm:pcm a)
+  (e:inames)
+  (r:ref a pcm)
+  (v0:FStar.Ghost.erased a)
+  (v1:FStar.Ghost.erased a{composable pcm v0 v1})
+: pst_ghost_action_except unit e
+    (pts_to r (v0 `op pcm` v1))
+    (fun _ -> pts_to r v0 `star` pts_to r v1)
+
+(** Combining separate permissions into a single composite permission *)
+val gather_action
+  (#a:Type u#a)
+  (#pcm:pcm a)
+  (e:inames)
+  (r:ref a pcm)
+  (v0:FStar.Ghost.erased a)
+  (v1:FStar.Ghost.erased a)
+: pst_ghost_action_except (squash (composable pcm v0 v1)) e
+    (pts_to r v0 `star` pts_to r v1)
+    (fun _ -> pts_to r (op pcm v0 v1))
+
+val alloc_action (#a:Type u#a) (#pcm:pcm a) (e:inames) (x:a{pcm.refine x})
+: pst_action_except (ref a pcm) e
+    emp
+    (fun r -> pts_to r x)
+
+val select_refine (#a:Type u#a) (#p:pcm a)
+                  (e:inames)
+                  (r:ref a p)
+                  (x:erased a)
+                  (f:(v:a{compatible p x v}
+                      -> GTot (y:a{compatible p y v /\
+                                  FStar.PCM.frame_compatible p x v y})))
+: pst_action_except (v:a{compatible p x v /\ p.refine v}) e
+    (pts_to r x)
+    (fun v -> pts_to r (f v))
+
+val upd_gen (#a:Type u#a) (#p:pcm a) (e:inames) (r:ref a p) (x y:Ghost.erased a)
+            (f:FStar.PCM.frame_preserving_upd p x y)
+: pst_action_except unit e
+    (pts_to r x)
+    (fun _ -> pts_to r y)
+
+val pts_to_not_null_action 
+      (#a:Type u#a) (#pcm:pcm a)
+      (e:inames)
+      (r:erased (ref a pcm))
+      (v:Ghost.erased a)
+: pst_ghost_action_except (squash (not (is_null r))) e
+    (pts_to r v)
+    (fun _ -> pts_to r v)
+
+(* Ghost references to "small" types *)
+[@@erasable]
+val core_ghost_ref : Type0
+let ghost_ref (#a:Type u#a) (p:pcm a) : Type0 = core_ghost_ref
+val ghost_pts_to (#a:Type u#a) (#p:pcm a) (r:ghost_ref p) (v:a) : vprop u#a
+
+val ghost_alloc
+    (#o:_)
+    (#a:Type u#a)
+    (#pcm:pcm a)
+    (x:erased a{pcm.refine x})
+: pst_ghost_action_except
+    (ghost_ref pcm)
+    o
+    emp 
+    (fun r -> ghost_pts_to r x)
+
+val ghost_read
+    #o
+    (#a:Type)
+    (#p:pcm a)
+    (r:ghost_ref p)
+    (x:erased a)
+    (f:(v:a{compatible p x v}
+        -> GTot (y:a{compatible p y v /\
+                     FStar.PCM.frame_compatible p x v y})))
+: pst_ghost_action_except
+    (erased (v:a{compatible p x v /\ p.refine v}))
+    o
+    (ghost_pts_to r x)
+    (fun v -> ghost_pts_to r (f v))
+
+val ghost_write
+    #o
+    (#a:Type)
+    (#p:pcm a)
+    (r:ghost_ref p)
+    (x y:Ghost.erased a)
+    (f:FStar.PCM.frame_preserving_upd p x y)
+: pst_ghost_action_except unit o 
+    (ghost_pts_to r x)
+    (fun _ -> ghost_pts_to r y)
+
+val ghost_share
+    #o
+    (#a:Type)
+    (#pcm:pcm a)
+    (r:ghost_ref pcm)
+    (v0:FStar.Ghost.erased a)
+    (v1:FStar.Ghost.erased a{composable pcm v0 v1})
+: pst_ghost_action_except unit o
+    (ghost_pts_to r (v0 `op pcm` v1))
+    (fun _ -> ghost_pts_to r v0 `star` ghost_pts_to r v1)
+
+val ghost_gather
+    #o
+    (#a:Type)
+    (#pcm:pcm a)
+    (r:ghost_ref pcm)
+    (v0:FStar.Ghost.erased a)
+    (v1:FStar.Ghost.erased a)
+: pst_ghost_action_except
+    (squash (composable pcm v0 v1)) o
+    (ghost_pts_to r v0 `star` ghost_pts_to r v1)
+    (fun _ -> ghost_pts_to r (op pcm v0 v1))
+
+(* Concrete references to "big" types *)
+val big_pts_to (#a:Type u#(a + 1)) (#pcm:_) (r:ref a pcm) (v:a) : big_vprop u#a
+
+val big_sel_action
+      (#a:Type u#(a + 1))
+      (#pcm:_)
+      (e:inames)
+      (r:ref a pcm)
+      (v0:erased a)
+: pst_action_except (v:a{compatible pcm v0 v}) e
+    (big_pts_to r v0)
+    (fun _ -> big_pts_to r v0)
+
+val big_upd_action
+      (#a:Type u#(a + 1)) (#pcm:_) (e:inames)
+      (r:ref a pcm)
+      (v0:FStar.Ghost.erased a)
+      (v1:a {FStar.PCM.frame_preserving pcm v0 v1 /\ pcm.refine v1})
+: pst_action_except unit e
+    (big_pts_to r v0)
+    (fun _ -> big_pts_to r v1)
+
+val big_free_action
+      (#a:Type u#(a + 1))
+      (#pcm:pcm a)
+      (e:inames)
+      (r:ref a pcm)
+      (x:FStar.Ghost.erased a{FStar.PCM.exclusive pcm x /\ pcm.refine pcm.FStar.PCM.p.one})
+: pst_action_except unit e
+    (big_pts_to r x)
+    (fun _ -> big_pts_to r pcm.FStar.PCM.p.one)
+
+(** Splitting a permission on a composite resource into two separate permissions *)
+val big_split_action
+      (#a:Type u#(a + 1))
+      (#pcm:pcm a)
+      (e:inames)
+      (r:ref a pcm)
+      (v0:FStar.Ghost.erased a)
+      (v1:FStar.Ghost.erased a{composable pcm v0 v1})
+: pst_ghost_action_except unit e
+    (big_pts_to r (v0 `op pcm` v1))
+    (fun _ -> big_pts_to r v0 `star` big_pts_to r v1)
+
+(** Combining separate permissions into a single composite permission *)
+val big_gather_action
+      (#a:Type u#(a + 1))
+      (#pcm:pcm a)
+      (e:inames)
+      (r:ref a pcm)
+      (v0:FStar.Ghost.erased a)
+      (v1:FStar.Ghost.erased a)
+: pst_ghost_action_except (squash (composable pcm v0 v1)) e
+    (big_pts_to r v0 `star` big_pts_to r v1)
+    (fun _ -> big_pts_to r (op pcm v0 v1))
+
+val big_alloc_action
+      (#a:Type u#(a + 1))
+      (#pcm:pcm a)
+      (e:inames)
+      (x:a{pcm.refine x})
+: pst_action_except (ref a pcm) e
+    emp
+    (fun r -> big_pts_to r x)
+
+val big_select_refine
+      (#a:Type u#(a + 1))
+      (#p:pcm a)
+      (e:inames)
+      (r:ref a p)
+      (x:erased a)
+      (f:(v:a{compatible p x v}
+          -> GTot (y:a{compatible p y v /\
+                      FStar.PCM.frame_compatible p x v y})))
+: pst_action_except (v:a{compatible p x v /\ p.refine v}) e
+    (big_pts_to r x)
+    (fun v -> big_pts_to r (f v))
+
+val big_upd_gen
+    (#a:Type u#(a + 1))
+    (#p:pcm a)
+    (e:inames)
+    (r:ref a p)
+    (x y:Ghost.erased a)
+    (f:FStar.PCM.frame_preserving_upd p x y)
+: pst_action_except unit e
+    (big_pts_to r x)
+    (fun _ -> big_pts_to r y)
+
+val big_pts_to_not_null_action 
+      (#a:Type u#(a + 1))
+      (#pcm:pcm a)
+      (e:inames)
+      (r:erased (ref a pcm))
+      (v:Ghost.erased a)
+: pst_ghost_action_except (squash (not (is_null r))) e
+    (big_pts_to r v)
+    (fun _ -> big_pts_to r v)
+
+(* Ghost references to "small" types *)
+val big_ghost_pts_to (#a:Type u#(a + 1)) (#p:pcm a) (r:ghost_ref p) (v:a) : big_vprop u#a
+
+val big_ghost_alloc
+    (#o:_)
+    (#a:Type u#(a + 1))
+    (#pcm:pcm a)
+    (x:erased a{pcm.refine x})
+: pst_ghost_action_except
+    (ghost_ref pcm)
+    o
+    emp 
+    (fun r -> big_ghost_pts_to r x)
+
+val big_ghost_read
+    #o
+    (#a:Type u#(a + 1))
+    (#p:pcm a)
+    (r:ghost_ref p)
+    (x:erased a)
+    (f:(v:a{compatible p x v}
+        -> GTot (y:a{compatible p y v /\
+                     FStar.PCM.frame_compatible p x v y})))
+: pst_ghost_action_except
+    (erased (v:a{compatible p x v /\ p.refine v}))
+    o
+    (big_ghost_pts_to r x)
+    (fun v -> big_ghost_pts_to r (f v))
+
+val big_ghost_write
+    #o
+    (#a:Type u#(a + 1))
+    (#p:pcm a)
+    (r:ghost_ref p)
+    (x y:Ghost.erased a)
+    (f:FStar.PCM.frame_preserving_upd p x y)
+: pst_ghost_action_except unit o 
+    (big_ghost_pts_to r x)
+    (fun _ -> big_ghost_pts_to r y)
+
+val big_ghost_share
+    #o
+    (#a:Type u#(a + 1))
+    (#pcm:pcm a)
+    (r:ghost_ref pcm)
+    (v0:FStar.Ghost.erased a)
+    (v1:FStar.Ghost.erased a{composable pcm v0 v1})
+: pst_ghost_action_except unit o
+    (big_ghost_pts_to r (v0 `op pcm` v1))
+    (fun _ -> big_ghost_pts_to r v0 `star` big_ghost_pts_to r v1)
+
+val big_ghost_gather
+    #o
+    (#a:Type u#(a + 1))
+    (#pcm:pcm a)
+    (r:ghost_ref pcm)
+    (v0:FStar.Ghost.erased a)
+    (v1:FStar.Ghost.erased a)
+: pst_ghost_action_except
+    (squash (composable pcm v0 v1)) o
+    (big_ghost_pts_to r v0 `star` big_ghost_pts_to r v1)
+    (fun _ -> big_ghost_pts_to r (op pcm v0 v1))
+
